src/Narcissus/BinLib/AlignedDomainName.v
@@ -1,0 +1,728 @@
+Require Import
+        Coq.Strings.String
+        Coq.Arith.Mult
+        Coq.Vectors.Vector.
+
+Require Import
+        Fiat.Common.BoundedLookup
+        Fiat.Common.ilist
+        Fiat.Common.DecideableEnsembles
+        Fiat.Common.StringFacts
+        Fiat.Computation
+        Fiat.Narcissus.Common.Specs
+        Fiat.Narcissus.Common.ComposeOpt
+        Fiat.Narcissus.Formats.WordOpt
+        Fiat.Narcissus.Formats.NatOpt
+        Fiat.Narcissus.Formats.StringOpt
+        Fiat.Narcissus.Formats.EnumOpt
+        Fiat.Narcissus.Formats.FixListOpt
+        Fiat.Narcissus.Formats.SumTypeOpt
+        Fiat.Narcissus.Formats.DomainNameOpt
+        Fiat.Narcissus.BinLib.AlignedByteString
+        Fiat.Narcissus.BinLib.AlignWord
+        Fiat.Narcissus.BinLib.AlignedDecoders
+        Fiat.Narcissus.BinLib.AlignedFix
+        Fiat.Common.IterateBoundedIndex
+        Fiat.Common.Tactics.CacheStringConstant
+        Fiat.Narcissus.Stores.DomainNameStore.
+
+Require Import
+        Bedrock.Word.
+
+Section AlignedDomainName.
+
+  Import Vectors.VectorDef.VectorNotations.
+
+  Arguments natToWord : simpl never.
+  Arguments wordToNat : simpl never.
+  Arguments NPeano.div : simpl never.
+  Opaque pow2. (* Don't want to be evaluating this. *)
+
+  Lemma split_string_OK
+    : forall d,
+      ValidDomainName d ->
+      (d = (fst (split_string (d)) ++ String "." (snd (split_string (d))))%string \/
+       split_string (d) = (d, ""%string)) /\
+      ValidLabel (fst (split_string (d))) /\
+      (forall label' post' : string,
+          d = (label' ++ post')%string ->
+          ValidLabel label' -> (String.length label' <= String.length (fst (split_string (d))))%nat).
+  Proof.
+  Admitted.
+
+  Lemma split_string_ValidDomainName :
+    forall d,
+      ValidDomainName d ->
+      ValidDomainName (snd (split_string d)).
+  Proof.
+  Admitted.
+
+  Lemma well_founded_string_length'
+    : well_founded (fun y r : {a : string & ValidDomainName a} => lt (String.length (projT1 y)) (String.length (projT1 r))%nat).
+  Proof.
+  Admitted.
+
+  Definition aligned_format_DomainName :=
+    Fix well_founded_string_length
+        (fun _ : string  =>
+           FixComp.LeastFixedPointFun.cfunType [CacheFormat] ({n : nat & t (word 8) n} * CacheFormat))
+        (fun (r : string)
+             (y : forall r' : string,
+                 lt (String.length r') (String.length r)%nat ->
+                 CacheFormat -> {n : nat & t (word 8) n} * CacheFormat)
+             (ce : CacheFormat) =>
+           match string_dec r "" with
+           | left e =>
+             (existT (fun n : nat => t (word 8) n) 1 [NToWord 8 (Ascii.N_of_ascii terminal_char)], addE ce 8)
+           | right e => (existT (fun n : nat => t (word 8) n)
+                                (1 + String.length (fst (split_string r)) +
+                                 projT1
+                                   (fst
+                                      (y
+                                         ((snd (split_string r)))
+                                         (@split_string_ValidDomainName_length r e)
+                                         (Ifopt Ifopt fst ce as m
+                                                                  Then if Compare_dec.lt_dec (wordToNat m + 8) (pow2 17)
+                                                                       then Some (natToWord 17 (wordToNat m + 8))
+                                                                       else None Else None as m
+                                                                                                Then if Compare_dec.lt_dec
+                                                                                                          (wordToNat m + 8 * String.length (fst (split_string r)))
+                                                                                                          (pow2 17)
+                                                                                                     then
+                                                                                                       Some (natToWord 17 (wordToNat m + 8 * String.length (fst (split_string r))))
+                                                                                                     else None Else None,
+                                                                                              snd ce))))
+                                (([natToWord 8 (String.length (let (x0, _) := split_string r in x0))] ++
+                                                                                                      StringToBytes (fst (split_string r))) ++
+                                                                                                                                            projT2
+                                                                                                                                            (fst
+                                                                                                                                               (y
+                                                                                                                                                  (snd (split_string r))
+                                                                                                                                                  (@split_string_ValidDomainName_length r e)
+                                                                                                                                                  (Ifopt Ifopt fst ce as m
+                                                                                                                                                                           Then if Compare_dec.lt_dec (wordToNat m + 8) (pow2 17)
+                                                                                                                                                                                then Some (natToWord 17 (wordToNat m + 8))
+                                                                                                                                                                                else None Else None as m
+                                                                                                                                                                                                         Then if Compare_dec.lt_dec
+                                                                                                                                                                                                                   (wordToNat m + 8 * String.length (fst (split_string r)))
+                                                                                                                                                                                                                   (pow2 17)
+                                                                                                                                                                                                              then
+                                                                                                                                                                                                                Some (natToWord 17 (wordToNat m + 8 * String.length (fst (split_string r))))
+                                                                                                                                                                                                              else None Else None,
+                                                                                                                                                                                                       snd ce)))),
+                         Ifopt Ifopt fst ce as m Then Some (Nat2pointerT (wordToNat (wtl (wtl (wtl m))))) Else None as curPtr
+                                                                                                                         Then (fst
+                                                                                                                                 (snd
+                                                                                                                                    (y
+                                                                                                                                       (snd (split_string r))
+                                                                                                                                       (@split_string_ValidDomainName_length r e)
+                                                                                                                                       (Ifopt Ifopt
+                                                                                                                                              fst ce as m
+                                                                                                                                                          Then if Compare_dec.lt_dec (wordToNat m + 8) (pow2 17)
+                                                                                                                                                               then Some (natToWord 17 (wordToNat m + 8))
+                                                                                                                                                               else None Else None as m
+                                                                                                                                                                                        Then if Compare_dec.lt_dec
+                                                                                                                                                                                                  (wordToNat m + 8 * String.length (fst (split_string r)))
+                                                                                                                                                                                                  (pow2 17)
+                                                                                                                                                                                             then
+                                                                                                                                                                                               Some (natToWord 17 (wordToNat m + 8 * String.length (fst (split_string r))))
+                                                                                                                                                                                             else None Else None,
+                                                                                                                                                                                      snd ce))),
+                                                                                                                               ((r, curPtr)
+                                                                                                                                  :: snd
+                                                                                                                                  (snd
+                                                                                                                                     (y (snd (split_string r))
+                                                                                                                                        (@split_string_ValidDomainName_length r e)
+                                                                                                                                        (Ifopt Ifopt
+                                                                                                                                               fst ce as m
+                                                                                                                                                           Then
+                                                                                                                                                           if Compare_dec.lt_dec (wordToNat m + 8) (pow2 17)
+                                                                                                                                                           then Some (natToWord 17 (wordToNat m + 8))
+                                                                                                                                                           else None Else None as m
+                                                                                                                                                                                    Then if Compare_dec.lt_dec
+                                                                                                                                                                                              (wordToNat m + 8 * String.length (fst (split_string r)))
+                                                                                                                                                                                              (pow2 17)
+                                                                                                                                                                                         then
+                                                                                                                                                                                           Some
+                                                                                                                                                                                             (natToWord 17 (wordToNat m + 8 * String.length (fst (split_string r))))
+                                                                                                                                                                                         else None Else None,
+                                                                                                                                                                                  snd ce))))%list)
+                                                                                                                         Else snd
+                                                                                                                         (y
+                                                                                                                            (snd (split_string r))
+                                                                                                                            (@split_string_ValidDomainName_length r e)
+                                                                                                                            (Ifopt Ifopt fst ce as m
+                                                                                                                                                     Then if Compare_dec.lt_dec (wordToNat m + 8) (pow2 17)
+                                                                                                                                                          then Some (natToWord 17 (wordToNat m + 8))
+                                                                                                                                                          else None Else None as m
+                                                                                                                                                                                   Then if Compare_dec.lt_dec
+                                                                                                                                                                                             (wordToNat m + 8 * String.length (fst (split_string r)))
+                                                                                                                                                                                             (pow2 17)
+                                                                                                                                                                                        then Some (natToWord 17 (wordToNat m + 8 * String.length (fst (split_string r))))
+                                                                                                                                                                                        else None Else None,
+                                                                                                                                                                                 snd ce)))
+           end).
+
+  Lemma refine_If_string_dec {A}
+    : forall s s' (t e : Comp A)
+             (t' : s = s' -> Comp A)
+             (e' : s <> s' -> Comp A),
+      (forall e'', refine t (t' e''))
+      -> (forall n, refine e (e' n))
+      -> refine (If string_dec s s' Then t Else e)
+                (match string_dec s s' with
+                 | left e'' => t' e''
+                 | right n => e' n
+                 end).
+  Proof.
+    intros; destruct (string_dec s s'); auto.
+  Qed.
+
+  Lemma align_format_DomainName
+    : forall d ce
+             (d_OK : ValidDomainName d),
+      refine (format_DomainName d ce)
+             (ret (build_aligned_ByteString (projT2 (fst (aligned_format_DomainName d ce))),
+                   (snd (aligned_format_DomainName d ce)))).
+  Proof.
+    intros.
+    etransitivity.
+    eapply (byte_align_Fix_encode_inv ValidDomainName) with
+    (lt_A := fun a a' => lt (String.length (projT1 a)) (String.length (projT1 a')));
+      eauto using format_body_monotone.
+    intros.
+    etransitivity.
+    match goal with
+      |- refine (If_Then_Else (bool_of_sumbool (string_dec ?s ?s')) _ _) _ =>
+      subst_refine_evar; eapply (refine_If_string_dec s s');
+        let H := fresh in
+        intro H; set_refine_evar; try rewrite H; simpl
+    end.
+    unfold AsciiOpt.format_ascii; rewrite aligned_format_char_eq.
+    subst_refine_evar; higher_order_reflexivity.
+    refine pick val None; try congruence.
+    simplify with monad laws; simpl.
+    unfold Bind2.
+    refine pick val (split_string (projT1 r)).
+    simplify with monad laws.
+    unfold format_nat.
+    rewrite aligned_format_char_eq.
+    simplify with monad laws.
+    rewrite format_string_ByteString.
+    simplify with monad laws.
+    unfold snd at 2; unfold snd at 2.
+    unfold fst at 2; unfold fst at 2.
+    unfold fst at 2.
+    rewrite (H (exist _ _ (split_string_ValidDomainName _ (projT2 r)))
+               (@split_string_ValidDomainName_length _ H0)).
+    simplify with monad laws.
+    Arguments mult : simpl never.
+    simpl.
+    subst_refine_evar; higher_order_reflexivity.
+    auto using addE_addE_plus.
+    destruct r; apply split_string_OK.
+    simpl; eauto.
+    instantiate (1 := (fun (r : {a : string & ValidDomainName a})
+                           (y : forall r' : {a : string & ValidDomainName a},
+                               lt (String.length (projT1 r')) (String.length (projT1 r))%nat ->
+                               CacheFormat -> {n : nat & t (word 8) n} * CacheFormat)
+                           (ce : CacheFormat) =>
+                         match string_dec (projT1 r) "" with
+                         | left _ =>  (existT (fun n : nat => t (word 8) n) 1 [NToWord 8 (Ascii.N_of_ascii terminal_char)], addE ce 8)
+                         | right n' =>  (existT (fun n : nat => t (word 8) n)
+                                                (1 + String.length (fst (split_string (projT1 r))) +
+                                                 projT1
+                                                   (fst
+                                                      (y
+                                                         (existT ValidDomainName
+                                                                 (snd (split_string (projT1 r)))
+                                                                 (split_string_ValidDomainName (projT1 r) (projT2 r)))
+                                                         (@split_string_ValidDomainName_length (projT1 r) n')
+                                                         (Ifopt Ifopt fst ce as m
+                                                                                  Then if Compare_dec.lt_dec (wordToNat m + 8) (pow2 17)
+                                                                                       then Some (natToWord 17 (wordToNat m + 8))
+                                                                                       else None Else None as m
+                                                                                                                Then if Compare_dec.lt_dec
+                                                                                                                          (wordToNat m + 8 * String.length (fst (split_string (projT1 r))))
+                                                                                                                          (pow2 17)
+                                                                                                                     then
+                                                                                                                       Some (natToWord 17 (wordToNat m + 8 * String.length (fst (split_string (projT1 r)))))
+                                                                                                                     else None Else None,
+                                                                                                              snd ce))))
+                                                (([natToWord 8 (String.length (let (x0, _) := split_string (projT1 r) in x0))] ++
+                                                                                                                               StringToBytes (fst (split_string (projT1 r)))) ++
+                                                                                                                                                                              projT2
+                                                                                                                                                                              (fst
+                                                                                                                                                                                 (y
+                                                                                                                                                                                    (existT ValidDomainName
+                                                                                                                                                                                            (snd (split_string (projT1 r)))
+                                                                                                                                                                                            (split_string_ValidDomainName (projT1 r) (projT2 r)))
+                                                                                                                                                                                    (@split_string_ValidDomainName_length (projT1 r) n')
+                                                                                                                                                                                    (Ifopt Ifopt fst ce as m
+                                                                                                                                                                                                             Then if Compare_dec.lt_dec (wordToNat m + 8) (pow2 17)
+                                                                                                                                                                                                                  then Some (natToWord 17 (wordToNat m + 8))
+                                                                                                                                                                                                                  else None Else None as m
+                                                                                                                                                                                                                                           Then if Compare_dec.lt_dec
+                                                                                                                                                                                                                                                     (wordToNat m + 8 * String.length (fst (split_string (projT1 r))))
+                                                                                                                                                                                                                                                     (pow2 17)
+                                                                                                                                                                                                                                                then
+                                                                                                                                                                                                                                                  Some (natToWord 17 (wordToNat m + 8 * String.length (fst (split_string (projT1 r)))))
+                                                                                                                                                                                                                                                else None Else None,
+                                                                                                                                                                                                                                         snd ce)))),
+                                         Ifopt Ifopt fst ce as m Then Some (Nat2pointerT (wordToNat (wtl (wtl (wtl m))))) Else None as curPtr
+                                                                                                                                         Then (fst
+                                                                                                                                                 (snd
+                                                                                                                                                    (y
+                                                                                                                                                       (existT ValidDomainName
+                                                                                                                                                               (snd (split_string (projT1 r)))
+                                                                                                                                                               (split_string_ValidDomainName (projT1 r) (projT2 r)))
+                                                                                                                                                       (@split_string_ValidDomainName_length (projT1 r) n')
+                                                                                                                                                       (Ifopt Ifopt
+                                                                                                                                                              fst ce as m
+                                                                                                                                                                          Then if Compare_dec.lt_dec (wordToNat m + 8) (pow2 17)
+                                                                                                                                                                               then Some (natToWord 17 (wordToNat m + 8))
+                                                                                                                                                                               else None Else None as m
+                                                                                                                                                                                                        Then if Compare_dec.lt_dec
+                                                                                                                                                                                                                  (wordToNat m + 8 * String.length (fst (split_string (projT1 r))))
+                                                                                                                                                                                                                  (pow2 17)
+                                                                                                                                                                                                             then
+                                                                                                                                                                                                               Some (natToWord 17 (wordToNat m + 8 * String.length (fst (split_string (projT1 r)))))
+                                                                                                                                                                                                             else None Else None,
+                                                                                                                                                                                                      snd ce))),
+                                                                                                                                               ((projT1 r, curPtr)
+                                                                                                                                                  :: snd
+                                                                                                                                                  (snd
+                                                                                                                                                     (y
+                                                                                                                                                        (existT ValidDomainName
+                                                                                                                                                                (snd (split_string (projT1 r)))
+                                                                                                                                                                (split_string_ValidDomainName (projT1 r) (projT2 r)))
+                                                                                                                                                        (@split_string_ValidDomainName_length (projT1 r) n')
+                                                                                                                                                        (Ifopt Ifopt
+                                                                                                                                                               fst ce as m
+                                                                                                                                                                           Then
+                                                                                                                                                                           if Compare_dec.lt_dec (wordToNat m + 8) (pow2 17)
+                                                                                                                                                                           then Some (natToWord 17 (wordToNat m + 8))
+                                                                                                                                                                           else None Else None as m
+                                                                                                                                                                                                    Then if Compare_dec.lt_dec
+                                                                                                                                                                                                              (wordToNat m + 8 * String.length (fst (split_string (projT1 r))))
+                                                                                                                                                                                                              (pow2 17)
+                                                                                                                                                                                                         then
+                                                                                                                                                                                                           Some
+                                                                                                                                                                                                             (natToWord 17 (wordToNat m + 8 * String.length (fst (split_string (projT1 r)))))
+                                                                                                                                                                                                         else None Else None,
+                                                                                                                                                                                                  snd ce))))%list)
+                                                                                                                                         Else snd
+                                                                                                                                         (y
+                                                                                                                                            (existT ValidDomainName
+                                                                                                                                                    (snd (split_string (projT1 r)))
+                                                                                                                                                    (split_string_ValidDomainName (projT1 r) (projT2 r)))
+                                                                                                                                            (@split_string_ValidDomainName_length (projT1 r) n')
+                                                                                                                                            (Ifopt Ifopt fst ce as m
+                                                                                                                                                                     Then if Compare_dec.lt_dec (wordToNat m + 8) (pow2 17)
+                                                                                                                                                                          then Some (natToWord 17 (wordToNat m + 8))
+                                                                                                                                                                          else None Else None as m
+                                                                                                                                                                                                   Then if Compare_dec.lt_dec
+                                                                                                                                                                                                             (wordToNat m + 8 * String.length (fst (split_string (projT1 r))))
+                                                                                                                                                                                                             (pow2 17)
+                                                                                                                                                                                                        then Some (natToWord 17 (wordToNat m + 8 * String.length (fst (split_string (projT1 r)))))
+                                                                                                                                                                                                        else None Else None,
+                                                                                                                                                                                                 snd ce))) end)).
+    simpl.
+    destruct (string_dec (projT1 r) ""); simpl.
+    reflexivity.
+    rewrite <- !build_aligned_ByteString_append.
+    destruct (y (existT ValidDomainName (snd (split_string (projT1 r))) (split_string_ValidDomainName (projT1 r) (projT2 r)))
+                (@split_string_ValidDomainName_length (projT1 r) n)
+                (Ifopt Ifopt fst ce0 as m
+                                          Then if Compare_dec.lt_dec (wordToNat m + 8) (pow2 17) then Some (natToWord 17 (wordToNat m + 8)) else None
+                                                                                                                                                   Else None as m
+                                                                                                                                                                  Then if Compare_dec.lt_dec (wordToNat m + 8 * String.length (fst (split_string (projT1 r)))) (pow2 17)
+                                                                                                                                                                       then Some (natToWord 17 (wordToNat m + 8 * String.length (fst (split_string (projT1 r)))))
+                                                                                                                                                                       else None Else None, snd ce0)); simpl.
+    rewrite <- !build_aligned_ByteString_append.
+    reflexivity.
+    intros; apply functional_extensionality; intros.
+    destruct (string_dec (projT1 x0) ""); simpl; try rewrite H; reflexivity.
+    instantiate (2 := well_founded_string_length').
+    instantiate (1 := d_OK).
+    match goal with
+      |- context [let (_,_) := ?z in _] =>
+      replace z with
+      (aligned_format_DomainName d ce)
+    end.
+    destruct (aligned_format_DomainName d ce); reflexivity.
+    simpl. admit.
+  Qed.
+
+  (*  Lemma align_format_DomainName
+    : forall d ce
+      (d_OK : ValidDomainName d),
+      refine (format_DomainName d ce)
+             (ret (build_aligned_ByteString (projT2 (fst (aligned_format_DomainName d ce))),
+                   (snd (aligned_format_DomainName d ce)))).
+  Proof.
+    intros.
+    etransitivity.
+    eapply (byte_align_Fix_encode_inv ValidDomainName) with
+    (lt_A := fun a a' => lt (String.length (projT1 a)) (String.length (projT1 a')));
+      eauto using format_body_monotone.
+    intros.
+    etransitivity.
+    match goal with
+      |- refine (If_Then_Else (bool_of_sumbool (string_dec ?s ?s')) _ _) _ =>
+      subst_refine_evar; eapply (refine_If_string_dec s s');
+        let H := fresh in
+        intro H; set_refine_evar; try rewrite H; simpl
+    end.
+    unfold AsciiOpt.format_ascii; rewrite aligned_format_char_eq.
+    subst_refine_evar; higher_order_reflexivity.
+    refine pick val None; try congruence.
+    simplify with monad laws; simpl.
+    unfold Bind2.
+    refine pick val (split_string (projT1 r)).
+    simplify with monad laws.
+    unfold format_nat.
+    rewrite aligned_format_char_eq.
+    simplify with monad laws.
+    rewrite format_string_ByteString.
+    simplify with monad laws.
+    unfold snd at 2; unfold snd at 2.
+    unfold fst at 2; unfold fst at 2.
+    unfold fst at 2.
+    rewrite (H (exist _ _ (split_string_ValidDomainName _ (projT2 r)))
+                   (@split_string_ValidDomainName_length _ H0)).
+    simplify with monad laws.
+    Arguments mult : simpl never.
+    simpl.
+    subst_refine_evar; higher_order_reflexivity.
+    auto using addE_addE_plus.
+    destruct r; apply split_string_OK.
+    simpl; eauto.
+    instantiate (1 := (fun (r : {a : string & ValidDomainName a})
+                     (y : forall r' : {a : string & ValidDomainName a},
+                          lt (String.length (projT1 r')) (String.length (projT1 r))%nat ->
+                          CacheFormat -> {n : nat & t (word 8) n} * CacheFormat)
+                     (ce : CacheFormat) =>
+                   match string_dec (projT1 r) "" with
+                   | left _ =>  (existT (fun n : nat => t (word 8) n) 1 [NToWord 8 (Ascii.N_of_ascii terminal_char)], addE ce 8)
+                   | right n' =>  (existT (fun n : nat => t (word 8) n)
+                           (1 + String.length (fst (split_string (projT1 r))) +
+                            projT1
+                              (fst
+                                 (y
+                                    (existT ValidDomainName
+                                       (snd (split_string (projT1 r)))
+                                       (split_string_ValidDomainName (projT1 r) (projT2 r)))
+                                    (@split_string_ValidDomainName_length (projT1 r) n')
+                                    (Ifopt Ifopt fst ce as m
+                                           Then if Compare_dec.lt_dec (wordToNat m + 8) (pow2 17)
+                                                then Some (natToWord 17 (wordToNat m + 8))
+                                                else None Else None as m
+                                     Then if Compare_dec.lt_dec
+                                               (wordToNat m + 8 * String.length (fst (split_string (projT1 r))))
+                                               (pow2 17)
+                                          then
+                                           Some (natToWord 17 (wordToNat m + 8 * String.length (fst (split_string (projT1 r)))))
+                                          else None Else None,
+                                    snd ce))))
+                           (([natToWord 8 (String.length (let (x0, _) := split_string (projT1 r) in x0))] ++
+                             StringToBytes (fst (split_string (projT1 r)))) ++
+                            projT2
+                              (fst
+                                 (y
+                                    (existT ValidDomainName
+                                       (snd (split_string (projT1 r)))
+                                       (split_string_ValidDomainName (projT1 r) (projT2 r)))
+                                    (@split_string_ValidDomainName_length (projT1 r) n')
+                                    (Ifopt Ifopt fst ce as m
+                                           Then if Compare_dec.lt_dec (wordToNat m + 8) (pow2 17)
+                                                then Some (natToWord 17 (wordToNat m + 8))
+                                                else None Else None as m
+                                     Then if Compare_dec.lt_dec
+                                               (wordToNat m + 8 * String.length (fst (split_string (projT1 r))))
+                                               (pow2 17)
+                                          then
+                                           Some (natToWord 17 (wordToNat m + 8 * String.length (fst (split_string (projT1 r)))))
+                                          else None Else None,
+                                    snd ce)))),
+                        Ifopt Ifopt fst ce as m Then Some (Nat2pointerT (wordToNat (wtl (wtl (wtl m))))) Else None as curPtr
+                        Then (fst
+                                (snd
+                                   (y
+                                      (existT ValidDomainName
+                                         (snd (split_string (projT1 r)))
+                                         (split_string_ValidDomainName (projT1 r) (projT2 r)))
+                                      (@split_string_ValidDomainName_length (projT1 r) n')
+                                      (Ifopt Ifopt
+                                             fst ce as m
+                                             Then if Compare_dec.lt_dec (wordToNat m + 8) (pow2 17)
+                                                  then Some (natToWord 17 (wordToNat m + 8))
+                                                  else None Else None as m
+                                       Then if Compare_dec.lt_dec
+                                                 (wordToNat m + 8 * String.length (fst (split_string (projT1 r))))
+                                                 (pow2 17)
+                                            then
+                                             Some (natToWord 17 (wordToNat m + 8 * String.length (fst (split_string (projT1 r)))))
+                                            else None Else None,
+                                      snd ce))),
+                             ((projT1 r, curPtr)
+                              :: snd
+                                   (snd
+                                      (y
+                                         (existT ValidDomainName
+                                            (snd (split_string (projT1 r)))
+                                            (split_string_ValidDomainName (projT1 r) (projT2 r)))
+                                         (@split_string_ValidDomainName_length (projT1 r) n')
+                                         (Ifopt Ifopt
+                                                fst ce as m
+                                                Then
+                                                if Compare_dec.lt_dec (wordToNat m + 8) (pow2 17)
+                                                then Some (natToWord 17 (wordToNat m + 8))
+                                                else None Else None as m
+                                          Then if Compare_dec.lt_dec
+                                                  (wordToNat m + 8 * String.length (fst (split_string (projT1 r))))
+                                                  (pow2 17)
+                                               then
+                                                Some
+                                                  (natToWord 17 (wordToNat m + 8 * String.length (fst (split_string (projT1 r)))))
+                                               else None Else None,
+                                         snd ce))))%list)
+                        Else snd
+                               (y
+                                  (existT ValidDomainName
+                                     (snd (split_string (projT1 r)))
+                                     (split_string_ValidDomainName (projT1 r) (projT2 r)))
+                                  (@split_string_ValidDomainName_length (projT1 r) n')
+                                  (Ifopt Ifopt fst ce as m
+                                         Then if Compare_dec.lt_dec (wordToNat m + 8) (pow2 17)
+                                              then Some (natToWord 17 (wordToNat m + 8))
+                                              else None Else None as m
+                                   Then if Compare_dec.lt_dec
+                                             (wordToNat m + 8 * String.length (fst (split_string (projT1 r))))
+                                             (pow2 17)
+                                        then Some (natToWord 17 (wordToNat m + 8 * String.length (fst (split_string (projT1 r)))))
+                                        else None Else None,
+                                  snd ce))) end)).
+    simpl.
+    destruct (string_dec (projT1 r) ""); simpl.
+    reflexivity.
+    rewrite <- !build_aligned_ByteString_append.
+    progress destruct (y (existT ValidDomainName (snd (split_string (projT1 r))) (split_string_ValidDomainName (projT1 r) (projT2 r)))
+                (@split_string_ValidDomainName_length (projT1 r) n)
+                (Ifopt Ifopt fst ce0 as m
+                       Then if Compare_dec.lt_dec (wordToNat m + 8) (pow2 17) then Some (natToWord 17 (wordToNat m + 8)) else None
+                       Else None as m
+                 Then if Compare_dec.lt_dec (wordToNat m + 8 * String.length (fst (split_string (projT1 r)))) (pow2 17)
+                      then Some (natToWord 17 (wordToNat m + 8 * String.length (fst (split_string (projT1 r)))))
+                      else None Else None, snd ce0)) eqn:?; simpl.
+    match goal with
+      |- context [y ?A ?B ?C] => set (H4 := y A B C)
+    end.
+  Admitted.
+   (*    rewrite Heqp in H4.
+    rewrite <- !build_aligned_ByteString_append.
+    reflexivity.
+    intros; apply functional_extensionality; intros.
+    destruct (string_dec (projT1 x0) ""); simpl; try rewrite H; reflexivity.
+    instantiate (2 := well_founded_string_length').
+    instantiate (1 := d_OK).
+    match goal with
+      |- context [let (_,_) := ?z in _] =>
+      replace z with
+      (aligned_format_DomainName d ce)
+    end.
+    destruct (aligned_format_DomainName d ce); reflexivity.
+    simpl. admit.
+  Qed. *) *)
+
+
+
+  Lemma byte_align_Fix_encode {A}
+        (lt_A : A -> A -> Prop)
+        (wf_lt_A : well_founded lt_A)
+    : forall
+      (body : FixComp.funType [A; CacheFormat] (ByteString * CacheFormat)
+              -> FixComp.funType [A; CacheFormat] (ByteString * CacheFormat))
+      (body' : forall r : A,
+          (forall r' : A, lt_A r' r -> FixComp.LeastFixedPointFun.cfunType [CacheFormat] ({n : _ & Vector.t (word 8) n} * CacheFormat)) ->
+          FixComp.LeastFixedPointFun.cfunType [CacheFormat] ({n : _ & Vector.t (word 8) n} * CacheFormat))
+
+      (refine_body_OK : forall (r : A)
+                               (x : A -> CacheFormat  ->
+                                    Comp (ByteString * CacheFormat))
+                               (y : forall r' : A,
+                                   lt_A r' r ->
+                                   CacheFormat ->
+                                   {n : _ & Vector.t (word 8) n} * CacheFormat),
+          (forall (a' : A) (wf_r : lt_A a' r) (ce : CacheFormat),
+              refine (x a' ce)
+                     (ret (let (v, ce') := y a' wf_r ce in
+                           (build_aligned_ByteString (projT2 v), ce'))))
+          -> forall ce, refine (body x r ce) (ret (let (v, ce') := body' r y ce in
+                                                   (build_aligned_ByteString (projT2 v), ce'))))
+
+      (body_monotone : forall rec rec' : FixComp.funType [A; CacheFormat] (ByteString * CacheFormat),
+          FixComp.refineFun rec rec' -> FixComp.refineFun (body rec) (body rec'))
+      (body'_monotone : forall (x0 : A)
+                               (f
+                                  g : {y : A | lt_A y x0} ->
+                                      CacheFormat ->
+                                      {n : nat & t (word 8) n} * (CacheFormat)),
+          (forall y : {y : A | lt_A y x0}, f y = g y) ->
+          body' x0 (fun (a' : A) (lt_a' : lt_A a' x0) => f (exist (fun a'0 : A => lt_A a'0 x0) a' lt_a')) =
+          body' x0 (fun (a' : A) (lt_a' : lt_A a' x0) => g (exist (fun a'0 : A => lt_A a'0 x0) a' lt_a')))
+      (a : A) (ce : CacheFormat),
+      refine (FixComp.LeastFixedPointFun.LeastFixedPoint body a ce)
+             (ret (let (v, ce') := Fix wf_lt_A _ body' a ce in
+                   (build_aligned_ByteString (projT2 v), ce'))).
+  Proof.
+    intros.
+    unfold FixComp.LeastFixedPointFun.LeastFixedPoint, respectful_hetero; intros.
+    simpl.
+    revert ce; pattern a; eapply (well_founded_ind wf_lt_A).
+    simpl; intros.
+    pose proof (proj1 (Frame.Is_GreatestFixedPoint (O := @FixComp.LeastFixedPointFun.funDefOps [A; CacheFormat] (ByteString * CacheFormat)) _ (body_monotone))); etransitivity.
+    eapply H0; eauto.
+    destruct (Fix wf_lt_A
+                  (fun _ : A =>
+                     CacheFormat ->
+                     {n : nat & t (word 8) n} * (CacheFormat)) body' x ce) eqn: ?.
+    pose proof (Fix_eq _ _ wf_lt_A _ (fun a rec => body' a (fun a' lt_a' => rec (existT (fun a' => lt_A a' a) a' lt_a')))).
+    generalize Heqp as Heqp'; intros.
+    simpl in H1; unfold Fix_sub, Fix_F_sub in H1; unfold Fix, Fix_F in Heqp.
+    rewrite H1 in Heqp; simpl in Heqp; clear H1; eauto.
+    etransitivity.
+    eapply refine_body_OK.
+    instantiate (1 := (fun (a' : A) (_ : lt_A a' x) =>
+                         (fix Fix_F_sub (x0 : A) (r : Acc lt_A x0) {struct r} :
+                            CacheFormat ->
+                            {n : nat & t (word 8) n} * (CacheFormat) :=
+                            body' x0 (fun (a'0 : A) (lt_a'0 : lt_A a'0 x0) => Fix_F_sub a'0 (Acc_inv r lt_a'0))) a'
+                                                                                                                 (wf_lt_A a'))).
+    eapply H; eauto.
+    unfold CacheFormat, dns_list_cache.
+    rewrite Heqp.
+    unfold CacheFormat, dns_list_cache in Heqp'.
+    rewrite Heqp'; reflexivity.
+  Qed.
+
+  Lemma byte_align_Fix_encode_inv {A}
+        (A_OK : A -> Prop)
+        (lt_A : _ -> _ -> Prop)
+        (wf_lt_A : well_founded lt_A)
+    : forall
+      (body : FixComp.funType [A; CacheFormat] (ByteString * CacheFormat)
+              -> FixComp.funType [A; CacheFormat] (ByteString * CacheFormat))
+      (body' : forall r : { a : _ & A_OK a},
+          (forall r' : { a : _ & A_OK a},
+              lt_A r' r
+              -> FixComp.LeastFixedPointFun.cfunType [CacheFormat] ({n : _ & Vector.t (word 8) n} * CacheFormat)) ->
+          FixComp.LeastFixedPointFun.cfunType [CacheFormat] ({n : _ & Vector.t (word 8) n} * CacheFormat))
+      (refine_body_OK : forall (r : { a : _ & A_OK a})
+                               (x : A -> CacheFormat ->
+                                    Comp (ByteString * CacheFormat))
+                               (y : forall r' : { a : _ & A_OK a},
+                                   lt_A r' r ->
+                                   CacheFormat ->
+                                   {n : _ & Vector.t (word 8) n} * CacheFormat),
+          (forall (a' : { a : _ & A_OK a}) (wf_r : lt_A a' r) (ce : CacheFormat),
+              refine (x (projT1 a') ce)
+                     (ret (let (v, ce') := y a' wf_r ce in
+                           (build_aligned_ByteString (projT2 v), ce'))))
+          -> forall ce, refine (body x (projT1 r) ce) (ret (let (v, ce') := body' r y ce in
+                                                            (build_aligned_ByteString (projT2 v), ce'))))
+
+      (body_monotone : forall rec rec' : FixComp.funType [A; CacheFormat] (ByteString * CacheFormat),
+          FixComp.refineFun rec rec' -> FixComp.refineFun (body rec) (body rec'))
+      (body'_monotone : forall (x0 : { a : _ & A_OK a})
+                               (f
+                                  g : {y : { a : _ & A_OK a} | lt_A y x0} ->
+                                      CacheFormat ->
+                                      {n : nat & t (word 8) n} * (CacheFormat)),
+          (forall y : {y : { a : _ & A_OK a} | lt_A y x0}, f y = g y) ->
+          body' x0 (fun (a' : { a : _ & A_OK a}) (lt_a' : lt_A a' x0) => f (exist (fun a'0 : { a : _ & A_OK a} => lt_A a'0 x0) a' lt_a')) =
+          body' x0 (fun (a' : { a : _ & A_OK a}) (lt_a' : lt_A a' x0) => g (exist (fun a'0 : { a : _ & A_OK a} => lt_A a'0 x0) a' lt_a')))
+      (a : A) (ce : CacheFormat) (a_OK : A_OK a),
+      refine (FixComp.LeastFixedPointFun.LeastFixedPoint body a ce)
+             (ret (let (v, ce') := Fix wf_lt_A _ body' (existT _ _ a_OK) ce in
+                   (build_aligned_ByteString (projT2 v), ce'))).
+  Proof.
+    intros.
+    unfold FixComp.LeastFixedPointFun.LeastFixedPoint, respectful_hetero; intros.
+    simpl.
+    replace a with (projT1 (existT _ a a_OK)) at 1.
+    revert ce; pattern (existT _ a a_OK); eapply (well_founded_ind wf_lt_A).
+    simpl; intros.
+    pose proof (proj1 (Frame.Is_GreatestFixedPoint (O := @FixComp.LeastFixedPointFun.funDefOps [A; CacheFormat] (ByteString * CacheFormat)) _ (body_monotone))); etransitivity.
+    eapply H0; eauto.
+    destruct ( Fix wf_lt_A
+                   (fun _ : {a0 : A & A_OK a0} =>
+                      CacheFormat ->
+                      {n : nat & t (word 8) n} * (CacheFormat)) body' x ce) eqn: ?.
+    pose proof (Fix_eq _ _ wf_lt_A _ (fun a rec => body' a (fun a' lt_a' => rec (existT (fun a' => lt_A a' a) a' lt_a')))).
+    simpl in H1; unfold Fix_sub, Fix_F_sub in H1; unfold Fix, Fix_F in Heqp.
+    generalize Heqp as Heqp'; intros.
+    rewrite H1 in Heqp; simpl in Heqp; clear H1; eauto.
+    etransitivity.
+    eapply refine_body_OK.
+    instantiate (1 := fun (a' : {a0 : A & A_OK a0}) (_ : lt_A a' x) =>
+                        (fix Fix_F_sub (x0 : {a0 : A & A_OK a0}) (r : Acc lt_A x0) {struct r} :
+                           CacheFormat ->
+                           {n : nat & t (word 8) n} * (CacheFormat) :=
+                           body' x0 (fun (a'0 : {a0 : A & A_OK a0}) (lt_a'0 : lt_A a'0 x0) => Fix_F_sub a'0 (Acc_inv r lt_a'0))) a'
+                                                                                                                                 (wf_lt_A a')).
+    eapply H; eauto.
+    unfold CacheFormat, dns_list_cache, Fix, Fix_F in *.
+    rewrite Heqp, Heqp'.
+    reflexivity.
+    reflexivity.
+  Qed.
+  (*intros. 8.6 script.
+    unfold FixComp.LeastFixedPointFun.LeastFixedPoint, respectful_hetero; intros.
+    simpl.
+    replace a with (projT1 (existT (fun a0 : A => A_OK a0) a a_OK)) at 1 by reflexivity.
+    revert ce; pattern (existT (fun a0 : A => A_OK a0) a a_OK); eapply (well_founded_ind wf_lt_A).
+    simpl; intros.
+    pose proof (proj1 (Frame.Is_GreatestFixedPoint (O := @FixComp.LeastFixedPointFun.funDefOps [A; CacheFormat] (ByteString * CacheFormat)) _ (body_monotone))); etransitivity.
+    eapply H0; eauto.
+    destruct (Fix wf_lt_A
+               (fun _ : {a0 : A & A_OK a0} =>
+                CacheFormat ->
+                {n : nat & t (word 8) n} * (CacheFormat)) body' x ce) eqn: ?.
+    pose proof (Fix_eq _ _ wf_lt_A _ (fun a rec => body' a (fun a' lt_a' => rec (existT (fun a' => lt_A a' a) a' lt_a')))).
+    simpl in H1; unfold Fix_sub, Fix_F_sub in H1; unfold Fix, Fix_F in Heqp.
+    rewrite H1 in Heqp; simpl in Heqp; clear H1; eauto.
+    etransitivity.
+    eapply refine_body_OK.
+    instantiate (1 := fun (a' : {a0 : A & A_OK a0}) (_ : lt_A a' x) =>
+            (fix Fix_F_sub (x0 : {a0 : A & A_OK a0}) (r : Acc lt_A x0) {struct r} :
+               CacheFormat ->
+               {n : nat & t (word 8) n} * (CacheFormat) :=
+               body' x0 (fun (a'0 : {a0 : A & A_OK a0}) (lt_a'0 : lt_A a'0 x0) => Fix_F_sub a'0 (Acc_inv r lt_a'0))) a'
+              (wf_lt_A a')).
+    simpl; intros; rewrite H; eauto;  reflexivity.
+    rewrite Heqp; try reflexivity. *)
+  (*Qed. *)
+
+  Lemma AlignedFormatDomainName
+    : (forall (ce : CacheFormat) (n m : nat), addE (addE ce n) m = addE ce (n + m)) ->
+      forall (numBytes : nat)
+             (d : DomainName)
+             (ce ce' : CacheFormat)
+             (c : CacheFormat -> Comp (ByteString * CacheFormat))
+             (v : t Core.char numBytes),
+        ValidDomainName d ->
+        refine (c (snd (aligned_format_DomainName d ce))) (ret (build_aligned_ByteString v, ce')) ->
+        refine ((format_DomainName d ThenC c) ce)
+               (ret (build_aligned_ByteString ((projT2 (fst (aligned_format_DomainName d ce))) ++ v), ce')).
+  Proof.
+    unfold compose at 1, Bind2; intros.
+    rewrite align_format_DomainName; eauto.
+    simplify with monad laws.
+    simpl; rewrite H1.
+    simplify with monad laws; simpl.
+    rewrite build_aligned_ByteString_append; reflexivity.
+  Qed.
+
+
+End AlignedDomainName.
