src/Narcissus/BinLib/AlignedFix.v
@@ -1,0 +1,185 @@
+Require Import
+        Coq.Strings.String
+        Coq.Arith.Mult
+        Coq.Vectors.Vector.
+
+Require Import
+        Fiat.Common.SumType
+        Fiat.Common.BoundedLookup
+        Fiat.Common.ilist
+        Fiat.Common.DecideableEnsembles
+        Fiat.Computation
+        Fiat.Narcissus.Common.Specs
+        Fiat.Narcissus.Common.ComposeOpt
+        Fiat.Narcissus.BinLib.AlignedByteString
+        Fiat.Narcissus.BinLib.AlignedDecoders.
+
+Require Import
+        Bedrock.Word.
+
+Section AlignedFix.
+
+  Context {cache : Cache}.
+  Context {cacheAddNat : CacheAdd cache nat}.
+
+  Lemma byte_align_Fix_encode {A}
+        (lt_A : A -> A -> Prop)
+        (wf_lt_A : well_founded lt_A)
+    : forall
+      (body : FixComp.funType [A; CacheFormat] (ByteString * CacheFormat)
+              -> FixComp.funType [A; CacheFormat] (ByteString * CacheFormat))
+      (body' : forall r : A,
+          (forall r' : A, lt_A r' r -> FixComp.LeastFixedPointFun.cfunType [CacheFormat] ({n : _ & Vector.t (word 8) n} * CacheFormat)) ->
+          FixComp.LeastFixedPointFun.cfunType [CacheFormat] ({n : _ & Vector.t (word 8) n} * CacheFormat))
+
+      (refine_body_OK : forall (r : A)
+                               (x : A -> CacheFormat  ->
+                                    Comp (ByteString * CacheFormat))
+                               (y : forall r' : A,
+                                   lt_A r' r ->
+                                   CacheFormat ->
+                                   {n : _ & Vector.t (word 8) n} * CacheFormat),
+          (forall (a' : A) (wf_r : lt_A a' r) (ce : CacheFormat),
+              refine (x a' ce)
+                     (ret (let (v, ce') := y a' wf_r ce in
+                           (build_aligned_ByteString (projT2 v), ce'))))
+          -> forall ce, refine (body x r ce) (ret (let (v, ce') := body' r y ce in
+                                                   (build_aligned_ByteString (projT2 v), ce'))))
+
+      (body_monotone : forall rec rec' : FixComp.funType [A; CacheFormat] (ByteString * CacheFormat),
+          FixComp.refineFun rec rec' -> FixComp.refineFun (body rec) (body rec'))
+      (body'_monotone : forall (x0 : A)
+                               (f
+                                  g : {y : A | lt_A y x0} ->
+                                      CacheFormat ->
+                                      {n : nat & t (word 8) n} * (CacheFormat)),
+          (forall y : {y : A | lt_A y x0}, f y = g y) ->
+          body' x0 (fun (a' : A) (lt_a' : lt_A a' x0) => f (exist (fun a'0 : A => lt_A a'0 x0) a' lt_a')) =
+          body' x0 (fun (a' : A) (lt_a' : lt_A a' x0) => g (exist (fun a'0 : A => lt_A a'0 x0) a' lt_a')))
+      (a : A) (ce : CacheFormat),
+      refine (FixComp.LeastFixedPointFun.LeastFixedPoint body a ce)
+             (ret (let (v, ce') := Fix wf_lt_A _ body' a ce in
+                   (build_aligned_ByteString (projT2 v), ce'))).
+  Proof.
+    intros.
+    unfold FixComp.LeastFixedPointFun.LeastFixedPoint, respectful_hetero; intros.
+    simpl.
+    revert ce; pattern a; eapply (well_founded_ind wf_lt_A).
+    simpl; intros.
+    pose proof (proj1 (Frame.Is_GreatestFixedPoint (O := @FixComp.LeastFixedPointFun.funDefOps [A; CacheFormat] (ByteString * CacheFormat)) _ (body_monotone))); etransitivity.
+    eapply H0; eauto.
+    destruct (Fix wf_lt_A
+                  (fun _ : A =>
+                     CacheFormat ->
+                     {n : nat & t (word 8) n} * (CacheFormat)) body' x ce) eqn: ?.
+    pose proof (Fix_eq _ _ wf_lt_A _ (fun a rec => body' a (fun a' lt_a' => rec (existT (fun a' => lt_A a' a) a' lt_a')))).
+    simpl in H1; unfold Fix_sub, Fix_F_sub in H1; unfold Fix, Fix_F in Heqp.
+    rewrite H1 in Heqp; simpl in Heqp; clear H1; eauto.
+    etransitivity.
+    eapply refine_body_OK.
+    instantiate (1 := (fun (a' : A) (_ : lt_A a' x) =>
+                         (fix Fix_F_sub (x0 : A) (r : Acc lt_A x0) {struct r} :
+                            CacheFormat ->
+                            {n : nat & t (word 8) n} * (CacheFormat) :=
+                            body' x0 (fun (a'0 : A) (lt_a'0 : lt_A a'0 x0) => Fix_F_sub a'0 (Acc_inv r lt_a'0))) a'
+                                                                                                                 (wf_lt_A a'))).
+    eapply H; eauto.
+    rewrite Heqp; reflexivity.
+  Qed.
+
+  Lemma byte_align_Fix_encode_inv {A}
+        (A_OK : A -> Prop)
+        (lt_A : _ -> _ -> Prop)
+        (wf_lt_A : well_founded lt_A)
+    : forall
+      (body : FixComp.funType [A; CacheFormat] (ByteString * CacheFormat)
+              -> FixComp.funType [A; CacheFormat] (ByteString * CacheFormat))
+      (body' : forall r : { a : _ & A_OK a},
+          (forall r' : { a : _ & A_OK a},
+              lt_A r' r
+              -> FixComp.LeastFixedPointFun.cfunType [CacheFormat] ({n : _ & Vector.t (word 8) n} * CacheFormat)) ->
+          FixComp.LeastFixedPointFun.cfunType [CacheFormat] ({n : _ & Vector.t (word 8) n} * CacheFormat))
+      (refine_body_OK : forall (r : { a : _ & A_OK a})
+                               (x : A -> CacheFormat ->
+                                    Comp (ByteString * CacheFormat))
+                               (y : forall r' : { a : _ & A_OK a},
+                                   lt_A r' r ->
+                                   CacheFormat ->
+                                   {n : _ & Vector.t (word 8) n} * CacheFormat),
+          (forall (a' : { a : _ & A_OK a}) (wf_r : lt_A a' r) (ce : CacheFormat),
+              refine (x (projT1 a') ce)
+                     (ret (let (v, ce') := y a' wf_r ce in
+                           (build_aligned_ByteString (projT2 v), ce'))))
+          -> forall ce, refine (body x (projT1 r) ce) (ret (let (v, ce') := body' r y ce in
+                                                            (build_aligned_ByteString (projT2 v), ce'))))
+
+      (body_monotone : forall rec rec' : FixComp.funType [A; CacheFormat] (ByteString * CacheFormat),
+          FixComp.refineFun rec rec' -> FixComp.refineFun (body rec) (body rec'))
+      (body'_monotone : forall (x0 : { a : _ & A_OK a})
+                               (f
+                                  g : {y : { a : _ & A_OK a} | lt_A y x0} ->
+                                      CacheFormat ->
+                                      {n : nat & t (word 8) n} * (CacheFormat)),
+          (forall y : {y : { a : _ & A_OK a} | lt_A y x0}, f y = g y) ->
+          body' x0 (fun (a' : { a : _ & A_OK a}) (lt_a' : lt_A a' x0) => f (exist (fun a'0 : { a : _ & A_OK a} => lt_A a'0 x0) a' lt_a')) =
+          body' x0 (fun (a' : { a : _ & A_OK a}) (lt_a' : lt_A a' x0) => g (exist (fun a'0 : { a : _ & A_OK a} => lt_A a'0 x0) a' lt_a')))
+      (a : A) (ce : CacheFormat) (a_OK : A_OK a),
+      refine (FixComp.LeastFixedPointFun.LeastFixedPoint body a ce)
+             (ret (let (v, ce') := Fix wf_lt_A _ body' (existT _ _ a_OK) ce in
+                   (build_aligned_ByteString (projT2 v), ce'))).
+  Proof.
+    intros.
+    unfold FixComp.LeastFixedPointFun.LeastFixedPoint, respectful_hetero; intros.
+    simpl.
+    replace a with (projT1 (existT _ a a_OK)) at 1.
+    revert ce; pattern (existT _ a a_OK); eapply (well_founded_ind wf_lt_A).
+    simpl; intros.
+    pose proof (proj1 (Frame.Is_GreatestFixedPoint (O := @FixComp.LeastFixedPointFun.funDefOps [A; CacheFormat] (ByteString * CacheFormat)) _ (body_monotone))); etransitivity.
+    eapply H0; eauto.
+    destruct ( Fix wf_lt_A
+                   (fun _ : {a0 : A & A_OK a0} =>
+                      CacheFormat ->
+                      {n : nat & t (word 8) n} * (CacheFormat)) body' x ce) eqn: ?.
+    pose proof (Fix_eq _ _ wf_lt_A _ (fun a rec => body' a (fun a' lt_a' => rec (existT (fun a' => lt_A a' a) a' lt_a')))).
+    simpl in H1; unfold Fix_sub, Fix_F_sub in H1; unfold Fix, Fix_F in Heqp.
+    rewrite H1 in Heqp; simpl in Heqp; clear H1; eauto.
+    etransitivity.
+    eapply refine_body_OK.
+    instantiate (1 := fun (a' : {a0 : A & A_OK a0}) (_ : lt_A a' x) =>
+                        (fix Fix_F_sub (x0 : {a0 : A & A_OK a0}) (r : Acc lt_A x0) {struct r} :
+                           CacheFormat ->
+                           {n : nat & t (word 8) n} * (CacheFormat) :=
+                           body' x0 (fun (a'0 : {a0 : A & A_OK a0}) (lt_a'0 : lt_A a'0 x0) => Fix_F_sub a'0 (Acc_inv r lt_a'0))) a'
+                                                                                                                                 (wf_lt_A a')).
+    eapply H; eauto.
+    rewrite Heqp; reflexivity.
+    reflexivity.
+  Qed.
+(*intros. 8.6 script.
+    unfold FixComp.LeastFixedPointFun.LeastFixedPoint, respectful_hetero; intros.
+    simpl.
+    replace a with (projT1 (existT (fun a0 : A => A_OK a0) a a_OK)) at 1 by reflexivity.
+    revert ce; pattern (existT (fun a0 : A => A_OK a0) a a_OK); eapply (well_founded_ind wf_lt_A).
+    simpl; intros.
+    pose proof (proj1 (Frame.Is_GreatestFixedPoint (O := @FixComp.LeastFixedPointFun.funDefOps [A; CacheFormat] (ByteString * CacheFormat)) _ (body_monotone))); etransitivity.
+    eapply H0; eauto.
+    destruct (Fix wf_lt_A
+               (fun _ : {a0 : A & A_OK a0} =>
+                CacheFormat ->
+                {n : nat & t (word 8) n} * (CacheFormat)) body' x ce) eqn: ?.
+    pose proof (Fix_eq _ _ wf_lt_A _ (fun a rec => body' a (fun a' lt_a' => rec (existT (fun a' => lt_A a' a) a' lt_a')))).
+    simpl in H1; unfold Fix_sub, Fix_F_sub in H1; unfold Fix, Fix_F in Heqp.
+    rewrite H1 in Heqp; simpl in Heqp; clear H1; eauto.
+    etransitivity.
+    eapply refine_body_OK.
+    instantiate (1 := fun (a' : {a0 : A & A_OK a0}) (_ : lt_A a' x) =>
+            (fix Fix_F_sub (x0 : {a0 : A & A_OK a0}) (r : Acc lt_A x0) {struct r} :
+               CacheFormat ->
+               {n : nat & t (word 8) n} * (CacheFormat) :=
+               body' x0 (fun (a'0 : {a0 : A & A_OK a0}) (lt_a'0 : lt_A a'0 x0) => Fix_F_sub a'0 (Acc_inv r lt_a'0))) a'
+              (wf_lt_A a')).
+    simpl; intros; rewrite H; eauto;  reflexivity.
+    rewrite Heqp; try reflexivity. *)
+  (*Qed. *)
+
+End AlignedFix.
