src/Narcissus/BinLib/AlignedList.v
@@ -1,0 +1,206 @@
+Require Import
+        Coq.Strings.String
+        Coq.Arith.Mult
+        Coq.Vectors.Vector.
+
+Require Import
+        Fiat.Common.SumType
+        Fiat.Common.BoundedLookup
+        Fiat.Common.ilist
+        Fiat.Common.DecideableEnsembles
+        Fiat.Computation
+        Fiat.Narcissus.Common.Specs
+        Fiat.Narcissus.Common.ComposeOpt
+        Fiat.Narcissus.Formats.WordOpt
+        Fiat.Narcissus.Formats.NatOpt
+        Fiat.Narcissus.Formats.StringOpt
+        Fiat.Narcissus.Formats.EnumOpt
+        Fiat.Narcissus.Formats.FixListOpt
+        Fiat.Narcissus.Formats.SumTypeOpt
+        Fiat.Narcissus.Formats.DomainNameOpt
+        Fiat.Narcissus.BinLib.AlignedByteString
+        Fiat.Narcissus.BinLib.AlignWord
+        Fiat.Narcissus.BinLib.AlignedDecoders
+        Fiat.Common.IterateBoundedIndex
+        Fiat.Common.Tactics.CacheStringConstant.
+
+Require Import
+        Bedrock.Word.
+
+Section AlignedList.
+
+  Context {cache : Cache}.
+  Context {cacheAddNat : CacheAdd cache nat}.
+
+  Fixpoint align_decode_list {A}
+           (A_decode_align : forall n,
+               Vector.t (word 8) n
+               -> CacheDecode
+               -> option (A * {n : _ & Vector.t _ n}
+                          * CacheDecode))
+           (n : nat)
+           {sz}
+           (v : Vector.t (word 8) sz)
+           (cd : CacheDecode)
+    : option (list A *  {n : _ & Vector.t _ n} * CacheDecode) :=
+    match n with
+    | 0 => Some (@nil _, existT _ _ v, cd)
+    | S s' => `(x, b1, e1) <- A_decode_align sz v cd;
+                `(xs, b2, e2) <- align_decode_list A_decode_align s' (projT2 b1) e1;
+                Some ((x :: xs)%list, b2, e2)
+    end.
+
+  Lemma optimize_align_decode_list
+        {A}
+        (A_decode :
+           ByteString
+           -> CacheDecode
+           -> option (A * ByteString * CacheDecode))
+        (A_decode_align : forall n,
+            Vector.t (word 8) n
+            -> CacheDecode
+            -> option (A * {n : _ & Vector.t _ n}
+                       * CacheDecode))
+        (A_decode_OK :
+           forall n (v : Vector.t _ n) cd,
+             A_decode (build_aligned_ByteString v) cd =
+             Ifopt A_decode_align n v cd as a Then
+                                              Some (fst (fst a), build_aligned_ByteString (projT2 (snd (fst a))), snd a)
+                                              Else
+                                              None)
+    : forall (n : nat)
+             {sz}
+             (v : Vector.t (word 8) sz)
+             (cd : CacheDecode),
+      decode_list A_decode n (build_aligned_ByteString v) cd =
+      Ifopt align_decode_list A_decode_align n v cd as a Then
+                                                         Some (fst (fst a), build_aligned_ByteString (projT2 (snd (fst a))), snd a)
+                                                         Else
+                                                         None.
+  Proof.
+    induction n; simpl; intros; eauto.
+    rewrite A_decode_OK.
+    rewrite (If_Opt_Then_Else_DecodeBindOpt).
+    destruct (A_decode_align sz v cd) as [ [ [? [? ?] ] ?]  | ]; simpl; eauto.
+    rewrite IHn.
+    rewrite (If_Opt_Then_Else_DecodeBindOpt).
+    destruct (align_decode_list A_decode_align n t c)
+      as [ [ [? [? ?] ] ?]  | ]; simpl; eauto.
+  Qed.
+
+  Fixpoint align_format_list {A}
+           (A_format_align :
+              A
+              ->  CacheFormat
+              -> {n : _ & Vector.t (word 8) n} * CacheFormat)
+           (As : list A)
+           (ce : CacheFormat)
+    : {n : _ & Vector.t (word 8) n} * CacheFormat :=
+    match As with
+    | nil => (existT _ _ (Vector.nil _), ce)
+    | a :: As' =>
+      let (b, ce') := A_format_align a ce in
+      let (b', ce'') := align_format_list A_format_align As' ce' in
+      (existT _ _ (append (projT2 b) (projT2 b')), ce'')
+    end.
+
+  Lemma optimize_align_format_list
+        {A}
+        (format_A : A -> CacheFormat -> Comp (ByteString * CacheFormat))
+        (A_format_align :
+           A
+           ->  CacheFormat
+           -> {n : _ & Vector.t (word 8) n} * CacheFormat)
+        (A_format_OK :
+           forall a ce,
+             refine (format_A a ce)
+                    (ret (let (v', ce') := A_format_align a ce in
+                          (build_aligned_ByteString (projT2 v'), ce'))))
+    : forall (As : list A)
+             (ce : CacheFormat),
+      refine (format_list format_A As ce)
+             (let (v', ce') := (align_format_list A_format_align As ce) in
+              ret (build_aligned_ByteString (projT2 v'), ce')).
+  Proof.
+    induction As; simpl; intros; simpl.
+    - simpl.
+      repeat f_equiv.
+      eapply ByteString_f_equal.
+      instantiate (1 := eq_refl _); reflexivity.
+      instantiate (1 := eq_refl _); reflexivity.
+    - unfold Bind2.
+      rewrite A_format_OK; simplify with monad laws.
+      rewrite IHAs.
+      destruct (A_format_align a ce); simpl.
+      destruct (align_format_list A_format_align As c);
+        simplify with monad laws.
+      simpl.
+      rewrite <- build_aligned_ByteString_append.
+      reflexivity.
+  Qed.
+
+  Lemma AlignedFormatListThenC {A}
+        format_A
+        (encode_A : A -> CacheFormat -> {n : nat & t (word 8) n} * CacheFormat)
+    : forall (l : list A) ce (c : _ -> Comp _)
+             (v' : _ -> {n : nat & t (word 8) n})
+             (ce' : _ -> CacheFormat),
+      (forall (a : A) (ce : CacheFormat),
+          refine (format_A a ce) (ret (let (v', ce') := encode_A a ce in (build_aligned_ByteString (projT2 v'), ce'))))
+      -> (forall v ce'',
+             format_list format_A l ce ↝ (v, ce'') ->
+             refine (c ce'') (ret (build_aligned_ByteString (projT2 (v' ce'')), ce' ce'')))
+      -> refine (((format_list format_A l)
+                    ThenC c) ce)
+                (ret (let (v, ce'') := align_format_list encode_A l ce in
+                      build_aligned_ByteString
+                        (Vector.append (projT2 v) (projT2 (v' ce''))),
+                      let (v, ce'') := align_format_list encode_A l ce in
+                      ce' ce'')).
+  Proof.
+    intros.
+    etransitivity.
+    eapply AlignedFormatThenC.
+    rewrite (optimize_align_format_list format_A encode_A); try eassumption.
+    match goal with
+      |- context [let (v, c) := ?z in ret (@?b v c)] =>
+      rewrite (zeta_inside_ret z _)
+    end.
+    rewrite zeta_to_fst; simpl.
+    instantiate (2 := fun ce => fst (_ ce)).
+    instantiate (1 := fun ce => snd (_ ce)).
+    simpl; reflexivity.
+    intros; eapply H0; eauto.
+    simpl.
+    rewrite !zeta_to_fst; simpl; reflexivity.
+  Qed.
+
+  Lemma AlignedFormatListDoneC {A}
+        format_A
+        (encode_An : A -> CacheFormat -> nat)
+        (encode_A1 : forall a ce,  t (word 8) (encode_An a ce))
+        (encode_A2 : A -> CacheFormat -> CacheFormat)
+    : forall (l : list A) ce,
+      (forall (a : A) (ce : CacheFormat),
+          refine (format_A a ce) (ret (build_aligned_ByteString (encode_A1 a ce), encode_A2 a ce)))
+      -> refine (((format_list format_A l) DoneC) ce)
+                (ret (build_aligned_ByteString (projT2 (fst (align_format_list (fun a ce => (existT _ _ (encode_A1 a ce), encode_A2 a ce)) l ce))),
+                      let (v, ce'') := align_format_list (fun a ce => (existT _ _ (encode_A1 a ce), encode_A2 a ce)) l ce in
+                      ce'')).
+  Proof.
+    intros.
+    etransitivity.
+    eapply AlignedFormatDoneC.
+    rewrite (optimize_align_format_list format_A (fun a ce => (existT _ _ (encode_A1 a ce), encode_A2 a ce))); try eassumption.
+    match goal with
+      |- context [let (v, c) := ?z in ret (@?b v c)] =>
+      rewrite (zeta_inside_ret z _)
+    end.
+    rewrite zeta_to_fst; simpl.
+    instantiate (2 := fun ce => fst (_ ce)).
+    instantiate (1 := fun ce => snd (_ ce)).
+    simpl; reflexivity.
+    intros; rewrite zeta_to_fst; simpl; reflexivity.
+  Qed.
+
+End AlignedList.
