src/Narcissus/BinLib/AlignedSumType.v
@@ -1,0 +1,80 @@
+Require Import
+        Coq.Strings.String
+        Coq.Arith.Mult
+        Coq.Vectors.Vector.
+
+Require Import
+        Fiat.Common.SumType
+        Fiat.Common.BoundedLookup
+        Fiat.Common.ilist
+        Fiat.Common.DecideableEnsembles
+        Fiat.Common.IterateBoundedIndex
+        Fiat.Computation
+        Fiat.Narcissus.Common.Specs
+        Fiat.Narcissus.Common.ComposeOpt
+        Fiat.Narcissus.Formats.SumTypeOpt
+        Fiat.Narcissus.BinLib.AlignedByteString
+        Fiat.Narcissus.BinLib.AlignedDecoders.
+
+Require Import
+        Bedrock.Word.
+
+Section AlignedSumType.
+
+  Context {cache : Cache}.
+  Context {cacheAddNat : CacheAdd cache nat}.
+
+  Lemma align_format_sumtype_OK_inv'
+        {m : nat}
+        {types : t Type m}
+        (A_OKs : SumType types -> Prop)
+        (align_encoders :
+           ilist (B := (fun T : Type => T -> CacheFormat -> ({n : _ & Vector.t (word 8) n} * (CacheFormat)))) types)
+        (encoders :
+           ilist (B := (fun T : Type => T -> CacheFormat -> Comp (ByteString * (CacheFormat)))) types)
+        (encoders_OK : forall idx t (ce : CacheFormat),
+            A_OKs (inj_SumType _ idx t)
+            -> refine (ith encoders idx t ce)
+                      (ret (build_aligned_ByteString (projT2 (fst (ith align_encoders idx t ce))),
+                            snd (ith align_encoders idx t ce))))
+    : forall (st : SumType types)
+             (ce : CacheFormat),
+      A_OKs st
+      -> refine (format_SumType types encoders st ce)
+                (ret (build_aligned_ByteString (projT2 (fst (align_format_sumtype align_encoders st ce))),
+                      (snd (align_format_sumtype align_encoders st ce)))).
+  Proof.
+    intros; unfold format_SumType, align_format_sumtype.
+    rewrite encoders_OK; eauto.
+    reflexivity.
+    rewrite inj_SumType_proj_inverse; eauto.
+  Qed.
+
+  Corollary align_format_sumtype_OK
+            {m : nat}
+            {types : t Type m}
+            (A_OKs : SumType types -> Prop)
+            (align_encoders :
+               ilist (B := (fun T : Type => T -> CacheFormat -> ({n : _ & Vector.t (word 8) n} * (CacheFormat)))) types)
+            (encoders :
+               ilist (B := (fun T : Type => T -> CacheFormat -> Comp (ByteString * (CacheFormat)))) types)
+            (encoders_OK : Iterate_Ensemble_BoundedIndex
+                             (fun idx => forall t (ce : CacheFormat),
+                                  A_OKs (inj_SumType _ idx t)
+                                  -> refine (ith encoders idx t ce)
+                                            (ret (build_aligned_ByteString (projT2 (fst (ith align_encoders idx t ce))),
+                                                  snd (ith align_encoders idx t ce)))))
+    : forall (st : SumType types)
+             (ce : CacheFormat),
+      A_OKs st
+      -> refine (format_SumType types encoders st ce)
+                (ret (build_aligned_ByteString (projT2 (fst (align_format_sumtype align_encoders st ce))),
+                      (snd (align_format_sumtype align_encoders st ce)))).
+  Proof.
+    intros; eapply align_format_sumtype_OK_inv'; intros.
+    eapply Iterate_Ensemble_BoundedIndex_equiv in encoders_OK.
+    apply encoders_OK; eauto.
+    eauto.
+  Qed.
+
+End AlignedSumType.
